tests/src/default.rs
@@ -1,0 +1,5 @@
+//@ [!lean] skip
+
+fn f25() {
+    let _: [u32; 25] = Default::default();
+}
