backends/lean/Aeneas/Std/Array/Array.lean
@@ -2,6 +2,7 @@
 import Aeneas.List
 import Aeneas.Progress.Init
 import Aeneas.Std.Array.Core
+import Aeneas.Std.Default
 
 namespace Aeneas.Std
 
@@ -241,5 +242,26 @@ theorem Array.setSlice!_getElem!_suffix {α} {n} [Inhabited α]
   (s.setSlice! i s')[j]! = s[j]! := by
   simp only [Array.setSlice!, Array.getElem!_Nat_eq]
   simp_lists
+
+/- [core::array::{core::default::Default for @Array<T, N>}#36::default]:
+   Source: '/rustc/library/core/src/array/mod.rs', lines 455:12-455:35
+   Name pattern: [core::array::{core::default::Default<[@T; @]>}::default] -/
+def core.default.DefaultArray.default {T : Type} {N : Usize} (defaultInst : core.default.Default T) : Result (Array T N) := do
+  let x ← defaultInst.default
+  .ok (Array.repeat N x)
+
+/- Trait implementation: [core::array::{core::default::Default for @Array<T, N>}#36]
+   Source: '/rustc/library/core/src/array/mod.rs', lines 454:8-454:52
+   Name pattern: [core::default::Default<[@T; @]>]
+
+   Remark: the `Default` instance actually doesn't exist for *any* const generic `N`,
+   but only for known values. This doesn't change the fact that we can factor the
+   instances out in the Lean model.
+ -/
+@[reducible]
+def core.default.DefaultArray {T : Type} {N : Usize}
+  (defaultInst : core.default.Default T) : core.default.Default (Array T N) := {
+  default := core.default.DefaultArray.default defaultInst
+}
 
 end Aeneas.Std
